haskell + agda + coq

haskell/QuickCheck.hs
@@ -1,0 +1,32 @@
+import Test.QuickCheck
+
+
+
+myList :: Arbitrary a => Gen [a]
+myList = oneof
+    [ return []
+    , (:) <$> arbitrary <*> myList
+    ]
+
+myList' :: Arbitrary a => Gen [a]
+myList' = frequency 
+    [ (1, return [])
+    , (4, (:) <$> arbitrary <*> myList')
+    ]
+
+-- sized :: (Int -> Gen a) -> Gen a
+
+flexList :: Arbitrary a => Gen [a]
+flexList = sized $ \n ->
+    frequency
+        [ (1, return [])
+        , (n, (:) <$> arbitrary <*> flexList)
+        ]
+
+main :: IO ()
+main = do
+    sample $ (flexList :: Gen [Int])
+
+
+
+
