haskell/lam/Syntax.hs
@@ -5,6 +5,8 @@ module  Syntax
     ,   app
     )   where
 
+import Test.QuickCheck
+
 import Variable (Var) 
 
 var :: Var -> Term
@@ -23,9 +25,17 @@ data Term_ a
     | Lam a (Term_ a)
     | App (Term_ a) (Term_ a)
 
+-- TODO : proper parsing and pretty printing 
 instance (Show  a) => Show (Term_ a) where
     show (Var v)    = show v
     show (Lam v t)  = "(\\" ++ show v ++ " -> " ++ show t ++ ")"
     show (App t s)  = "("   ++ show t ++ " "    ++ show s ++ ")"
 
+-- TODO : something better than this
+instance (Arbitrary a) => Arbitrary (Term_ a) where
+    arbitrary = frequency 
+        [ (1, Var <$> arbitrary)
+        , (1, Lam <$> arbitrary <*> arbitrary)
+        , (1, App <$> arbitrary <*> arbitrary)
+        ]
 
