haskell/quickcheck.hs
@@ -1,6 +1,0 @@
-import Test.QuickCheck
-
-f :: [Integer] -> Bool
-f x = True
-
-
