coq/cpdt/coind_sem.v
@@ -52,7 +52,7 @@ CoInductive evalCmd : Env -> Cmd -> Env -> Prop :=
         evalCmd e1 (CWhile e c) e3
 .
 
-(* Need to build a coinduction principle for evalCmd *)
+(* Need to build a coinduction principle for evalCmd        *)
 Theorem evalCmd_coind : forall (R:Env -> Cmd -> Env -> Prop),
     (forall (e1 e2:Env) (e:Exp) (v:Var), 
         R e1 (CAssign v e) e2 -> e2 = update e1 v (evalExp e1 e))    ->
@@ -64,6 +64,39 @@ Theorem evalCmd_coind : forall (R:Env -> Cmd -> Env -> Prop),
             evalExp e1 e <> 0 /\ R e1 c e2 /\ R e2 (CWhile e c) e3)) ->
     (forall (e1 e2:Env) (c:Cmd), R e1 c e2 -> evalCmd e1 c e2).
 Proof.
-    intros R. intros H1.
+    intros R H1 H2 H3. cofix. intros e1 e2 c H. destruct c.
+    - apply H1 in H. rewrite H. constructor.
+    - rename e2 into e3. apply H2 in H. destruct H as [e2 [H12 H23]].
+      apply EvalSeq with e2; apply evalCmd_coind; assumption.
+    - rename e2 into e3. apply H3 in H. destruct H as [H|H].
+        + destruct H as [E1 E2]. subst. apply EvalWhileFalse. assumption.
+        + destruct H as [e2 [E1 [E2 E3]]]. apply EvalWhileTrue with e2.
+            { assumption. }
+            { apply evalCmd_coind. assumption. }
+            { apply evalCmd_coind. assumption. }
+Qed.
+
+Fixpoint optExp (e:Exp) : Exp :=
+    match e with
+    | EPlus (EConst 0) e    => optExp e
+    | EPlus e1 e2           => EPlus (optExp e1) (optExp e2)
+    | _                     => e
+    end.
+
+Fixpoint optCmd (c:Cmd) : Cmd :=
+    match c with
+    | CAssign v e   => CAssign v (optExp e)
+    | CSeq c1 c2    => CSeq (optCmd c1) (optCmd c2)
+    | CWhile e c    => CWhile (optExp e) (optCmd c)
+    end. 
+
+Lemma optExp_correct : forall (env:Env) (e:Exp), 
+    evalExp env (optExp e) = evalExp env e. 
+Proof.
+    intros env. induction e as [n|v|e1 IH1 e2 IH2].
+    - reflexivity.
+    - reflexivity.
+    - 
+
 
 Show.
