agda/id.agda
@@ -1,0 +1,16 @@
+module id where
+
+data _≡_ {ℓ} {X : Set ℓ} : X → X → Set ℓ where
+  refl : (x : X) -> x ≡ x
+
+infixr 4 _≡_
+
+≡-refl : ∀{ℓ} {X : Set ℓ} (x : X) → x ≡ x
+≡-refl x = refl _
+
+≡-sym : ∀{ℓ} {X : Set ℓ} {x y : X} → x ≡ y → y ≡ x
+≡-sym (refl x) = refl _
+
+≡-trans : ∀ {ℓ} {X : Set ℓ} {x y z : X} → x ≡ y → y ≡ z → x ≡ z
+≡-trans (refl x) (refl y) = refl x
+
